Use simplified Stack functions. see #486

src/dafny/core/stack.dfy
@@ -17,7 +17,7 @@ module Stack {
     import opened Int
 
     // Maximum stack capcity is 1024 words.
-    const CAPACITY : int := 1024;
+    const CAPACITY: nat := 1024;
 
     type ValidStackContent = xs: seq<u256> | |xs| <= CAPACITY
 
@@ -93,92 +93,17 @@ module Stack {
 
     }
 
-    // A raw stack consistents of a sequence of data, and a stack pointer.
-    // datatype Raw = Stack(contents:seq<u256>)
-
-    // A valid Stack cannot exceed the capacity.
-    // type T = s:Raw | |s.contents| <= CAPACITY
-    // witness Stack([])
-    // type T = Stack 
-
+    //  The empty stack.
     const Empty := Stack(contents := [])
 
-    // Get number of items currently on this Stack.
-    function method Size(st: Stack) : nat { |st.contents| }
-
-    // Get remaining capacity of stack (i.e. number of items we could still
-    // push).
-    function method Capacity(st: Stack) : nat {
-      CAPACITY - |st.contents|
+    function method Make(xs: seq<u256>): Stack
+        requires |xs| <= CAPACITY {
+            Stack(contents := xs)
     }
 
-    // Create an empty stack.
-    function method Create() : Stack { Stack(contents:=[]) }
-
-    /** Make a stack with some initial contents.  */
-    function method Make(s: seq<u256>) : Stack 
-        requires |s| <= CAPACITY
-    {
-        Stack(contents:=s)
+    function method Create(): Stack
+     {
+            Stack(contents := [])
     }
 
-    // Push word onto Stack.  This requires that there is sufficient space for
-    // that item.
-    function method Push(st: Stack, val:u256) : Stack 
-        // Sanity check enough space.
-        requires Size(st) < CAPACITY {
-            Stack(contents:=([val] + st.contents))
-    }
-
-    // Peek nth word from top of Stack (where 0 is top item, 1 is next item, and
-    // so on).  This requires there are sufficiently many words.
-    function method Peek(st: Stack, k:int) : u256
-        // Sanity check enough items to pop!
-        requires k >= 0 && k < Size(st) {
-            st.contents[k]
-    }
-
-    // Peek top N words on the Stack.  This requires there are sufficiently many
-    // words.
-    function method PeekN(st: Stack, n:nat) : (r:seq<u256>)
-    requires Size(st) >= n
-    ensures |r| == n {
-            st.contents[0..n]
-    }
-
-    // Pop word off of this Stack.  This requires something to pop!
-    function method Pop(st: Stack) : Stack 
-        // Sanity check something to pop.
-        requires Size(st) > 0 {
-            Stack(contents:=st.contents[1..])
-    }
-
-    // Pop N words off of this Stack.  This requires something to pop!
-    function method PopN(st: Stack, n:nat) : Stack 
-        // Sanity check something to pop.
-        requires Size(st) >= n {
-            Stack(contents:=st.contents[n..])
-    }
-
-    /** Swap top item at index 0 and the k+1-th item at index k. */
-    function method Swap(st: Stack, k:nat) : Stack 
-      requires Size(st) > k > 0
-    {
-        var top := st.contents[0];
-        var kth := st.contents[k];
-        Stack(contents:=st.contents[0:=kth][k:=top])
-    }
-
-    /**
-     *  A sliced stack.
-     *  @param  st  A stack.
-     *  @param  l   An index.
-     *  @param  u   An index.
-     *  @returns    The stack made of the first u elements minus the first l.
-     */
-    function Slice(st: Stack, l: nat, u: nat): (r: Stack)
-        requires l <= u <= Size(st)
-    {
-        Stack(st.contents[l..u])
-    }
 }
